ex6Script.sml
@@ -1,0 +1,328 @@
+(*
+Copyright 2021 DeepMind Technologies Limited.
+
+Licensed under the Apache License, Version 2.0 (the "License");
+you may not use this file except in compliance with the License.
+You may obtain a copy of the License at
+
+    https://www.apache.org/licenses/LICENSE-2.0
+
+Unless required by applicable law or agreed to in writing, software
+distributed under the License is distributed on an "AS IS" BASIS,
+WITHOUT WARRANTIES OR CONDITIONS OF ANY KIND, either express or implied.
+See the License for the specific language governing permissions and
+limitations under the License.
+*)
+
+open HolKernel boolLib bossLib Parse dep_rewrite
+  pairTheory pred_setTheory categoryTheory
+  cf0Theory cf1Theory cf2Theory cf4Theory cf5Theory cf6Theory
+
+val _ = new_theory"ex6";
+
+Definition guests_def:
+  guests = {"J";"K";"L"}
+End
+
+Theorem FINITE_guests[simp]:
+  FINITE guests
+Proof
+  rw[guests_def]
+QED
+
+Definition party_world_def:
+  party_world = IMAGE encode_set (POW guests)
+End
+
+Theorem FINITE_party_world[simp]:
+  FINITE party_world
+Proof
+  rw[party_world_def]
+QED
+
+Definition guest_def:
+  guest x = mk_cf <| world := party_world;
+    agent := IMAGE encode_set (POW {x});
+    env := IMAGE encode_set (POW (guests DELETE x));
+    eval := λa e. encode_set (decode_set a ∪ decode_set e) |>
+End
+
+Definition jack_def:
+  jack = guest "J"
+End
+
+Definition kate_def:
+  kate = guest "K"
+End
+
+Definition luke_def:
+  luke = guest "L"
+End
+
+Theorem guest_in_chu_objects[simp]:
+  x ∈ guests ⇒
+  guest x ∈ chu_objects party_world
+Proof
+  rw[guest_def, in_chu_objects, finite_cf_def]
+  \\ rw[image_def, SUBSET_DEF]
+  \\ DEP_REWRITE_TAC[decode_encode_set]
+  \\ fs[IN_POW]
+  \\ conj_tac >- metis_tac[SUBSET_FINITE, FINITE_DELETE, FINITE_SING, FINITE_guests]
+  \\ simp[party_world_def]
+  \\ qmatch_goalsub_abbrev_tac`encode_set s`
+  \\ qexists_tac`s` \\ simp[Abbr`s`, IN_POW]
+  \\ fs[SUBSET_DEF]
+QED
+
+Theorem guest_world[simp]:
+  (guest x).world = party_world
+Proof
+  rw[guest_def]
+QED
+
+Theorem guest_eval:
+  (guest x).eval a e =
+  if a ∈ (guest x).agent ∧ e ∈ (guest x).env then
+    encode_set (decode_set a ∪ decode_set e)
+  else ARB
+Proof
+  rw[guest_def, mk_cf_def]
+QED
+
+Definition mor1_def:
+  mor1 x y = mk_chu_morphism (guest x) (swap (guest y))
+    <| map_agent := λa. if a = encode_set ∅ then a else encode_set {x};
+       map_env := λe. if e = encode_set ∅ then e else encode_set {y} |>
+End
+
+Definition mor2_def:
+  mor2 x y = mk_chu_morphism (guest x) (swap (guest y))
+    <| map_agent := λa. if a = encode_set ∅
+                            then encode_set (guests DIFF {x; y})
+                            else encode_set (guests DIFF {y});
+        map_env := λe. if e = encode_set ∅
+                          then encode_set (guests DIFF {x; y})
+                          else encode_set (guests DIFF {x}) |>
+End
+
+Theorem mor1_dom_cod[simp]:
+  (mor1 x y).dom = guest x ∧
+  (mor1 x y).cod = swap(guest y)
+Proof
+  rw[mor1_def]
+QED
+
+Theorem mor2_dom_cod[simp]:
+  (mor2 x y).dom = guest x ∧
+  (mor2 x y).cod = swap(guest y)
+Proof
+  rw[mor2_def]
+QED
+
+Theorem mor1_maps_to:
+  x ∈ guests ∧ y ∈ guests ∧ x ≠ y ⇒
+  mor1 x y :- guest x → swap (guest y) -: chu party_world
+Proof
+  rw[maps_to_in_chu, mor1_def]
+  \\ simp[mk_chu_morphism_def, is_chu_morphism_def]
+  \\ simp[restrict_def]
+  \\ simp[guest_def, PULL_EXISTS]
+  \\ simp[mk_cf_def]
+  \\ dsimp[POW_EQNS]
+  \\ qexistsl_tac[`{y}`,`{}`,`{x}`,`{}`]
+  \\ simp[]
+  \\ conj_asm1_tac >- simp[IN_POW]
+  \\ conj_asm1_tac >- simp[IN_POW]
+  \\ reverse IF_CASES_TAC >- metis_tac[]
+  \\ reverse IF_CASES_TAC >- metis_tac[]
+  \\ reverse IF_CASES_TAC >- metis_tac[IN_POW, EMPTY_SUBSET]
+  \\ reverse IF_CASES_TAC >- metis_tac[IN_POW, EMPTY_SUBSET]
+  \\ simp[UNION_COMM]
+QED
+
+Theorem mor2_maps_to:
+  x ∈ guests ∧ y ∈ guests ∧ x ≠ y ⇒
+  mor2 x y :- guest x → swap (guest y) -: chu party_world
+Proof
+  rw[maps_to_in_chu, mor2_def]
+  \\ simp[mk_chu_morphism_def, is_chu_morphism_def]
+  \\ simp[restrict_def]
+  \\ simp[guest_def, PULL_EXISTS]
+  \\ simp[mk_cf_def]
+  \\ dsimp[POW_EQNS]
+  \\ qexistsl_tac[`guests DIFF {x}`,`guests DIFF {x;y}`,
+                  `guests DIFF {y}`,`guests DIFF {x;y}`]
+  \\ simp[]
+  \\ conj_asm1_tac >- simp[IN_POW, SUBSET_DEF]
+  \\ conj_asm1_tac >- simp[IN_POW, SUBSET_DEF]
+  \\ reverse IF_CASES_TAC >- metis_tac[]
+  \\ reverse IF_CASES_TAC >- metis_tac[]
+  \\ reverse IF_CASES_TAC >- metis_tac[]
+  \\ reverse IF_CASES_TAC >- metis_tac[]
+  \\ simp[]
+  \\ simp[Once EXTENSION, GSYM CONJ_ASSOC]
+  \\ conj_tac >- metis_tac[]
+  \\ simp[Once EXTENSION]
+  \\ conj_tac >- metis_tac[]
+  \\ simp[Once EXTENSION]
+  \\ metis_tac[]
+QED
+
+Theorem maps_to_swap_guest:
+  x ∈ guests ∧ y ∈ guests ∧ x ≠ y ⇒
+  (m :- guest x → swap (guest y) -: chu party_world ⇔
+   m ∈ {mor1 x y; mor2 x y})
+Proof
+  strip_tac
+  \\ simp[]
+  \\ reverse eq_tac >- metis_tac[mor1_maps_to, mor2_maps_to]
+  \\ simp[maps_to_in_chu]
+  \\ simp[is_chu_morphism_def]
+  \\ strip_tac
+  \\ simp[morphism_component_equality]
+  \\ fs[guest_def, PULL_EXISTS]
+  \\ ntac 2 (pop_assum kall_tac)
+  \\ fs[mk_cf_def]
+  \\ fs[POW_EQNS]
+  \\ pop_assum mp_tac \\ dsimp[]
+  \\ ntac 2 (pop_assum mp_tac) \\ dsimp[]
+  \\ rpt gen_tac
+  \\ ntac 2 strip_tac
+  \\ DEP_REWRITE_TAC[decode_encode_set]
+  \\ fs[IN_POW]
+  \\ conj_asm1_tac
+  >- metis_tac [IN_POW, SUBSET_FINITE, FINITE_DELETE, FINITE_guests]
+  \\ simp[]
+  \\ strip_tac
+  \\ rpt BasicProvers.VAR_EQ_TAC \\ fs[]
+  \\ fs[extensional_def]
+  \\ simp[chu_morphism_map_component_equality]
+  \\ simp[FUN_EQ_THM, PULL_FORALL]
+  \\ simp[mor1_def, mor2_def, mk_chu_morphism_def]
+  \\ simp[guest_def, restrict_def, PULL_EXISTS, POW_EQNS]
+  \\ dsimp[]
+  \\ qmatch_assum_rename_tac`z ⊆ _`
+  \\ Cases_on`z = {}` \\ fs[]
+  >- ( disj1_tac \\ rw[] \\ metis_tac[] )
+  \\ `z = guests DIFF {x; y}`
+  by (
+    fs[SUBSET_DEF, GSYM MEMBER_NOT_EMPTY]
+    \\ simp[EXTENSION]
+    \\ gvs[guests_def]
+    \\ metis_tac[])
+  \\ disj2_tac
+  \\ rw[] \\ rw[]
+  \\ rw[EXTENSION]
+  \\ metis_tac[]
+QED
+
+Theorem mor1_neq_mor2:
+  mor1 x y ≠ mor2 x y
+Proof
+  rw[mor1_def, mor2_def, morphism_component_equality]
+  \\ rw[chu_morphism_map_component_equality]
+  \\ fs[mk_chu_morphism_def]
+  \\ fs[restrict_def]
+  \\ fs[FUN_EQ_THM]
+  \\ dsimp[guest_def, POW_EQNS]
+  \\ qexists_tac`encode_set ∅`
+  \\ simp[]
+  \\ simp[guests_def]
+  \\ rw[]
+QED
+
+Theorem tensor_guests_iso:
+  x ∈ guests ∧ y ∈ guests ∧ x ≠ y ⇒
+  tensor (guest x) (guest y) ≅
+    (swap (guest (CHOICE (guests DIFF {x;y})))) -: chu party_world
+Proof
+  rw[iso_objs_thm]
+  \\ qmatch_goalsub_abbrev_tac`swap (guest z)`
+  \\ qexists_tac`mk_chu_morphism (tensor (guest x) (guest y)) (swap (guest z))
+       <| map_agent := λp. let (a,b) = decode_pair p in
+            encode_set (decode_set a ∪ decode_set b);
+          map_env := λe.
+          encode_morphism
+            ((if e = encode_set ∅ then mor1 else mor2) x y )|>`
+  \\ `z ∈ guests ∧ z ≠ x ∧ z ≠ y`
+  by (
+    simp[Abbr`z`]
+    \\ qmatch_goalsub_abbrev_tac`CHOICE s`
+    \\ `CHOICE s ∈ s`
+    by(
+      irule CHOICE_DEF
+      \\ simp[Abbr`s`, GSYM MEMBER_NOT_EMPTY]
+      \\ gs[guests_def]
+      \\ dsimp[])
+    \\ fs[Abbr`s`])
+  \\ `guests = {x;y;z}`
+  by ( fs[guests_def] \\ gvs[]
+       \\ rw[EXTENSION] \\ metis_tac[])
+  \\ conj_asm1_tac
+  >- (
+    simp[maps_to_in_chu]
+    \\ simp[is_chu_morphism_def, mk_chu_morphism_def]
+    \\ simp[restrict_def]
+    \\ conj_asm1_tac
+    >- (
+      dsimp[tensor_def, hom_def] \\ rw[]
+      \\ metis_tac[mor1_maps_to, mor2_maps_to] )
+    \\ conj_asm1_tac
+    >- (
+      simp[tensor_def, PULL_EXISTS, EXISTS_PROD]
+      \\ simp[guest_def, PULL_EXISTS]
+      \\ dsimp[POW_EQNS]
+      \\ qexists_tac`{x}∪{y}`
+      \\ qexists_tac`{x}`
+      \\ qexists_tac`{y}`
+      \\ qexists_tac`{}` \\ simp[]
+      \\ simp[IN_POW, SUBSET_DEF])
+    \\ simp[tensor_eval]
+    \\ simp[tensor_def, PULL_EXISTS, EXISTS_PROD]
+    \\ simp[Ntimes guest_def 2, PULL_EXISTS]
+    \\ rpt gen_tac
+    \\ DEP_REWRITE_TAC[Q.GEN`w`decode_encode_chu_morphism]
+    \\ conj_tac >- metis_tac[mor1_maps_to, mor2_maps_to]
+    \\ simp[guest_eval]
+    \\ simp[guest_def, PULL_EXISTS]
+    \\ simp[DELETE_INSERT]
+    \\ dsimp[POW_EQNS]
+    \\ simp[mor1_def, mor2_def, mk_chu_morphism_def, restrict_def, guest_def]
+    \\ dsimp[POW_EQNS]
+    \\ rw[] \\ rw[] \\ gs[]
+    \\ fs[EXTENSION] \\ metis_tac[] )
+  \\ simp[chu_iso_bij]
+  \\ fs[maps_to_in_chu]
+  \\ fs[is_chu_morphism_def, mk_chu_morphism_def]
+  \\ fs[restrict_def]
+  \\ simp[BIJ_DEF, INJ_DEF, SURJ_DEF]
+  \\ simp[tensor_def, PULL_EXISTS, EXISTS_PROD]
+  \\ simp[Ntimes guest_def 9, hom_def, PULL_EXISTS]
+  \\ qpat_assum`_ = guests`(SUBST1_TAC o SYM)
+  \\ simp[DELETE_INSERT]
+  \\ dsimp[POW_EQNS]
+  \\ rpt disj1_tac
+  \\ conj_tac >- (simp[EXTENSION] \\ metis_tac[])
+  \\ conj_tac >- metis_tac[decode_encode_chu_morphism,
+                           mor1_neq_mor2, mor1_maps_to, mor2_maps_to]
+  \\ rpt strip_tac
+  \\ drule_then (drule_then (drule_then
+       (drule_then mp_tac o
+        Q.GEN`m` o #1 o EQ_IMP_RULE o SPEC_ALL))) maps_to_swap_guest
+  \\ dsimp[]
+  \\ simp[guest_def, PULL_EXISTS]
+  \\ dsimp[POW_EQNS]
+QED
+
+Theorem tensor_jack_kate:
+  tensor jack kate ≅ swap luke -: chu party_world
+Proof
+  rw[jack_def, kate_def, luke_def]
+  \\ `"L" = CHOICE (guests DIFF {"J";"K"})`
+  by simp[guests_def]
+  \\ pop_assum SUBST1_TAC
+  \\ irule tensor_guests_iso
+  \\ simp[guests_def]
+QED
+
+val _ = export_theory();
